Fixed some of the proofs after OCAP change.
There are problems with rewriting, that were not present before the
changes. Here are relevant SO-threads:

http://stackoverflow.com/questions/33028580/abstracting-over-the-term-leads-to-a-term-which-is-ill-typed

http://stackoverflow.com/questions/14867685/abstracting-leads-to-a-term-ill-typed-yet-well-typed

I wrote theorems heap_typeof_same, heap_typeof_impl in
heap.v (heap_typeof_same is admitted) and changed the proofs to use them
in several cases.

heap.v
@@ -7,7 +7,7 @@ Import ConcreteEverything.
 
 Section Heap.
   Variable P: Program.
-  Definition fieldsP := fields.
+  Definition fieldsP := fields P.
   Definition subclassP := subclass P.
   Definition fldP := fld P.
   Definition ftypeP := ftype P.
@@ -23,21 +23,62 @@ Section Heap.
   Definition heap_typeof (H: Heap_type) (o: Ref_type)
              (witn: In o (p_heap.domain H)) :
     class.
-    set (lem := proj2 (p_heap.fDomainCompat H o)).
+
+    assert ({b | p_heap.func H o = Some b}) as exists_value.
     case_eq (p_heap.func H o).
-    intros;    destruct b;    exact c.
-    intro is_none; set (is_absurd := lem is_none); firstorder.
+
+    intros b _; exists b; reflexivity.
+    intro is_none; induction (proj2 (p_heap.fDomainCompat _ _) is_none witn).
+    
+    destruct exists_value.
+    destruct x.
+    exact c.
+  Defined.
+  
+  Definition test_match n :=
+    match n with
+      | O => True
+      | S _ => True
+    end.
+
+  Theorem test_match_proof n :
+    test_match n = True.
+    destruct n; reflexivity.
   Defined.
 
+  
+  Theorem heap_typeof_same (H: Heap_type) (o: Ref_type) C FM :
+    p_heap.func H o = Some (obj C FM) ->
+    forall witn,
+      heap_typeof H o witn = C.
+    intros;
+    unfold heap_typeof;
+    destruct H;
+    unfold p_heap.func;
+    simpl in *;
+    compute.
+    admit.
+  Admitted.
 
-  (* Definition heap_type H o (o_witn: In o (p_heap.domain H)) : ClassName_type. *)
-  (*   set (lem := proj2 (p_heap.fDomainCompat H o)). *)
-  (*   case_eq (p_heap.func H o). *)
-  (*   intros. *)
-  (*   destruct b. *)
-  (*   exact c. *)
-  (*   intro is_none; elim ((lem is_none) o_witn). *)
-  (* Defined. *)
+  Theorem heap_typeof_impl H o C :
+    forall witn,
+      heap_typeof H o witn = C->
+      {FM | p_heap.func H o = Some (obj C FM)}.
+    intros.
+    case_eq (p_heap.func H o).
+    intros.
+    destruct b.
+    rewrite (heap_typeof_same H o c f H1 witn) in H0.
+    rewrite H0 in *; clear H0 c.
+    exists f; reflexivity.
+
+    (* None *)
+    intro is_none; induction (proj2 (p_heap.fDomainCompat _ _) is_none witn).
+  Qed.    
+    
+
+  Hint Resolve heap_typeof_same : Hints.
+  Hint Resolve heap_typeof_impl : Hints.
 
   Definition Heap_obj_ok H C FM :=
     forall f o,
